Proof of down_up identity with an arbitrary list of buffers passed

src/test/interop/Interop.fst
@@ -56,78 +56,6 @@ assume val lemma_upd_commute (#a:Type) (#rel:Preorder.preorder a) (h:HS.mem) (r1
                   HS.upd (HS.upd h r2 y) r1 x))
      [SMTPat (HS.upd (HS.upd h r1 x) r2 y)]
 
-(**
-
-TODO : This was the more generic version taking a variable number of parameters
-
-(* Takes a Hyperstack and a buffer, and updates a low-level Vale heap
-   with the contents of the buffer *)
-val update_vale_mem: HS.mem -> P.(buffer (TBase TUInt8)) -> Vale_Sem.heap -> GTot Vale_Sem.heap
-
-let update_vale_mem mem buf heap =
-  let addr = P.buffer_as_addr buf in
-  let length = P.buffer_length buf in
-  let contents = P.buffer_as_seq mem buf in
-  let rec aux (i:nat{i <= UInt32.v length}) curr_heap : GTot Vale_Sem.heap (decreases %[sub length i]) =
-    if i >= (UInt32.v length) then curr_heap
-    else
-      aux (i+1) (curr_heap.[addr + i] <- FStar.Seq.index contents i)
-  in aux 0 heap
-
-(* Copy write_buffer from FStar.Pointer.Base, replacing Stack effect by Tot *)
-assume val write_buffer
-  (#t: P.typ)
-  (b: P.buffer t)
-  (i: UInt32.t)
-  (v: P.type_of_typ t)
-  (mem: HS.mem)
-  : HS.mem
-
-assume val write_spec
-  (#t: P.typ)
-  (b: P.buffer t)
-  (i: UInt32.t)
-  (v: P.type_of_typ t)
-  (mem: HS.mem) : Lemma 
-  (requires UInt32.v i < UInt32.v (P.buffer_length b))
-  (ensures Seq.index (P.buffer_as_seq (write_buffer #t b i v mem) b) (UInt32.v i) == v )
-
-(* Takes a buffer, the previous HyperStack, and a low-level Vale Heap, and reconstructs the buffer
-   from the data in the Vale Heap *)
-val reconstruct_buf: P.(buffer (TBase TUInt8)) -> HS.mem -> Vale_Sem.heap -> GTot HS.mem
-let reconstruct_buf buf mem heap =
-  let addr = P.buffer_as_addr buf in
-  let length = P.buffer_length buf in
-  let rec aux (i:nat{i <= UInt32.v length}) curr_mem : GTot HS.mem (decreases %[sub length i]) =
-    if i >= (UInt32.v length) then curr_mem
-    else
-      aux (i+1) (write_buffer buf (UInt32.uint_to_t i) heap.[addr + i] curr_mem)
-  in aux 0 mem
-
-(* Takes a Low* Hyperstack, and a list of live buffers, and returns a low-level Vale heap
-containing these buffers *)
-val down_mem_list: HS.mem -> list P.(buffer (TBase TUInt8)) -> GTot Vale_Sem.heap
-
-let down_mem_list mem buffers =
-  (* Create a dummy heap *)
-  let heap : heap = FStar.Map.const (UInt8.uint_to_t 0) in
-  let heap = heap.[0] <- (UInt8.uint_to_t 1) in
-  let rec aux bufs accu_heap : GTot (Vale_Sem.heap) = match bufs with
-  | [] -> accu_heap
-  | a :: q -> aux q (update_vale_mem mem a accu_heap)
-  in aux buffers heap
-  
-(* Takes a low-level Vale Heap and the initial Hyperstack, and reconstructs the buffers in the HyperStack *)
-val up_mem_list: Vale_Sem.heap -> list P.(buffer (TBase TUInt8)) -> HS.mem -> GTot HS.mem
-
-let up_mem_list heap buffers mem =
-  let rec aux bufs accu_mem heap : GTot HS.mem = match bufs with
-    | [] -> accu_mem
-    | a :: q -> aux q (reconstruct_buf a accu_mem heap) heap
-  in aux buffers mem heap
-
-**)
-
 (* Write a buffer in the vale memory *)
 
 let rec write_vale_mem contents (length:nat{length = FStar.Seq.Base.length contents}) addr (i:nat{i <= length}) 
@@ -351,8 +279,8 @@ val up_mem: (heap:Vale_Sem.heap) -> (addrs:addr_map) -> (ptrs: list (B.buffer UI
 
 #set-options "--z3rlimit 100 --z3refresh"
 
-let up_mem heap addrs ptrs mem =
-  let rec aux (ps:list (B.buffer UInt8.t)) (accu: list (B.buffer UInt8.t){forall p. List.memP p ptrs <==> List.memP p ps \/ List.memP p accu}) 
+let rec up_mem_aux (heap:Vale_Sem.heap) (addrs:addr_map) (ptrs: list (B.buffer UInt8.t){list_disjoint_or_eq ptrs}) (ps:list (B.buffer UInt8.t))
+    (accu: list (B.buffer UInt8.t){forall p. List.memP p ptrs <==> List.memP p ps \/ List.memP p accu}) 
     (m:HS.mem{list_live m ps /\ list_live m accu /\ correct_up addrs accu m heap}) : GTot (new_mem:HS.mem{correct_up addrs ptrs new_mem heap}) = 
   match ps with
     | [] -> m
@@ -364,29 +292,33 @@ let up_mem heap addrs ptrs mem =
       correct_up_p_cancel heap addrs a m;
       correct_up_p_frame heap addrs a m;
       assert (forall p. List.memP p accu ==> disjoint_or_eq p a);
-      aux q (a::accu) new_mem
-  in
-  aux ptrs [] mem
+      up_mem_aux heap addrs ptrs q (a::accu) new_mem
 
-val down_up_identity: (mem:HS.mem) -> (addrs:addr_map) -> (ptr1:(B.buffer UInt8.t){B.live mem ptr1})  -> (ptr2:(B.buffer UInt8.t){B.live mem ptr2 /\ disjoint_or_eq ptr1 ptr2}) -> Lemma 
-  (let heap = down_mem mem addrs ptr1 ptr2 in 
-   let length1 = B.length ptr1 in
-   let length2 = B.length ptr2 in
-   let addr1 = addrs.[(B.as_addr ptr1, B.idx ptr1, B.length ptr1)] in
-   let addr2 = addrs.[(B.as_addr ptr2, B.idx ptr2, B.length ptr2)] in     
-   let new_mem = up_mem heap addrs ptr1 ptr2 mem in
+let up_mem heap addrs ptrs mem =  up_mem_aux heap addrs ptrs ptrs [] mem
+
+let rec invariant_up_mem_aux (heap:Vale_Sem.heap) (addrs:addr_map) (ptrs: list (B.buffer UInt8.t){list_disjoint_or_eq ptrs}) (ps:list (B.buffer UInt8.t))
+    (accu: list (B.buffer UInt8.t){forall p. List.memP p ptrs <==> List.memP p ps \/ List.memP p accu}) 
+    (m:HS.mem{list_live m ps /\ list_live m accu /\ correct_up addrs accu m heap}) : Lemma
+  (requires (forall b. List.memP b ptrs ==> (forall i. 0 <= i /\ i < B.length b ==> Seq.index (B.as_seq m b) i == heap.[addrs.[(B.as_addr b, B.idx b, B.length b)] + i])))
+  (ensures (m == up_mem_aux heap addrs ptrs ps accu m)) 
+  [SMTPat (m == up_mem_aux heap addrs ptrs ps accu m)] =
+  match ps with 
+    | [] -> ()
+    | a::q ->  
+      let length = B.length a in
+      let addr = addrs.[(B.as_addr a, B.idx a, B.length a)] in
+      let new_mem = write_low_mem heap length addr a m in
+      invariant_write_low_mem heap length addr a m;
+      invariant_up_mem_aux heap addrs ptrs q (a::accu) new_mem
+
+val down_up_identity: (mem:HS.mem) -> (addrs:addr_map) -> (ptrs:list (B.buffer UInt8.t){list_disjoint_or_eq ptrs /\ list_live mem ptrs }) -> Lemma 
+  (let heap = down_mem mem addrs ptrs in 
+   let new_mem = up_mem heap addrs ptrs mem in
     mem == new_mem)
-  
-let down_up_identity mem addrs ptr1 ptr2 =
-  let heap = down_mem mem addrs ptr1 ptr2 in 
-  let new_mem = up_mem heap addrs ptr1 ptr2 mem in
-  let length1 = B.length ptr1 in
-  let length2 = B.length ptr2 in
-  let addr1 = addrs.[(B.as_addr ptr1, B.idx ptr1, B.length ptr1)] in
-  let addr2 = addrs.[(B.as_addr ptr2, B.idx ptr2, B.length ptr2)] in   
-  let b1 = B.content ptr1 in
-  let b2 = B.content ptr2 in
-  invariant_write_low_mem heap length1 addr1 ptr1 mem;
-  let mem1 = write_low_mem heap length1 addr1 ptr1 mem in
-  invariant_write_low_mem heap length2 addr2 ptr2 mem;
+
+let down_up_identity mem addrs ptrs =
+  let heap = down_mem mem addrs ptrs in 
+  let new_mem = up_mem heap addrs ptrs mem in
+  assert (forall (p:B.buffer UInt8.t{List.memP p ptrs}). correct_up_p addrs mem heap p);
+  invariant_up_mem_aux heap addrs ptrs ptrs [] mem;
   ()
